multiple changes... - fixed some type mismatches related to Trace.event_g. - uncommented Trace.init to reveal expected kind/type mismatch with Subtrace.transform.

src/ghost/trace.fst
@@ -28,25 +28,49 @@ module Tesseract.Ghost.Trace
 
    type _event_g (key_t: Type) (substate_t: Type) (subevent_t: Type) =
       | Spawn: 
-         key: key_t -> step: Subtrace.transform_g substate_t subevent_t 
-            -> substate0: substate_t 
-            -> _event_g key_t substate_t subevent_t
+         key: key_t 
+         -> step: Subtrace.transform_g substate_t subevent_t 
+         -> substate0: substate_t 
+         -> _event_g key_t substate_t subevent_t
       | Service: 
-         key: key_t -> subevent: subevent_t 
-            -> _event_g key_t substate_t subevent_t
+         key: key_t 
+         -> subevent: subevent_t 
+         -> _event_g key_t substate_t subevent_t
 
    type is_event_safe: 
-      #key_t: Type -> #substate_t: Type -> #subevent_t: Type
-         -> state: state_g key_t substate_t subevent_t -> event: _event_g key_t substate_t subevent_t
-         -> Type =
-      fun (key_t: Type) (substate_t: Type) (subevent_t: Type) state event ->
-         // spawn events may only be issued when the actor isn't yet in the set of spawned actors.
-         (is_Spawn event ==> not (Map.is_mem state.children (Spawn.key event)))
-         /\ // service events may only be issued when the actor is already in the set of spawned actors.
-            (is_Service event ==> Map.is_mem state.children (Service.key event))
+      #key_t: Type 
+      -> #substate_t: Type 
+      -> #subevent_t: Type
+      -> state: state_g key_t substate_t subevent_t 
+      -> event: _event_g key_t substate_t subevent_t
+      -> Type 
+      = fun 
+            (key_t: Type) 
+            (substate_t: Type) 
+            (subevent_t: Type) 
+            state 
+            event 
+         ->
+            // spawn events may only be issued when the actor isn't yet in the set of spawned actors.
+            (is_Spawn event ==> not (Map.is_mem state.children (Spawn.key event)))
+            /\ // service events may only be issued when the actor is already in the set of spawned actors.
+               (is_Service event ==> Map.is_mem state.children (Service.key event))
 
-   (*type event_g (key_t: Type) (substate_t: Type) (subevent_t: Type) (state: state_g key_t substate_t subevent_t) =
-      state: state_g key_t substate_t subevent_t -> event: _event_g key_t substate_t subevent_t{is_event_safe state event}*)
+   type event_g:
+      key_t: Type 
+      -> substate_t: Type 
+      -> subevent_t: Type 
+      -> state_g key_t substate_t subevent_t 
+      -> Type 
+      = fun 
+            (key_t: Type)
+            (substate_t: Type)
+            (subevent_t: Type)
+            (state: 
+               state_g key_t substate_t subevent_t)
+         -> 
+            event: 
+               _event_g key_t substate_t subevent_t{is_event_safe state event}
 
    type trace_g (key_t: Type) (substate_t: Type) (subevent_t: Type) = 
       Subtrace.subtrace_g
@@ -54,41 +78,54 @@ module Tesseract.Ghost.Trace
          (_event_g key_t substate_t subevent_t) 
 
    val transform: 
-      #key_t: Type -> #substate_t: Type -> #subevent_t: Type 
-         -> state: state_g key_t substate_t subevent_t
-         -> event: _event_g key_t substate_t subevent_t{is_event_safe state event}
-         -> Tot (state_g key_t substate_t subevent_t)
+      #key_t: Type 
+      -> #substate_t: Type 
+      -> #subevent_t: Type 
+      -> state: state_g key_t substate_t subevent_t
+      -> event: 
+            _event_g key_t substate_t subevent_t{is_event_safe state event}
+      //-> event: event_g key_t substate_t subevent_t state
+      -> Tot (state_g key_t substate_t subevent_t)
    let transform 
-      (key_t: Type) (substate_t: Type) (subevent_t: Type) 
-      state event =
-         let ordinal' = state.ordinal + 1 in
-            match event with
-               | Spawn key xform substate ->
-                  {
-                     ordinal = ordinal';
-                     children = 
-                        Map.add state.children key (substate, xform)
-                  }
-               | Service key subevent ->
-                  (match Map.lookup state.children key with
-                     | (substate, xform) ->
-                        let substate' = xform substate subevent in
-                           {
-                              ordinal = ordinal';
-                              children = 
-                                 Map.subst state.children key (substate', xform)
-                           })
+      (key_t: Type) 
+      (substate_t: Type) 
+      (subevent_t: Type) 
+      state 
+      event 
+      = let ordinal' = state.ordinal + 1 in
+         match event with
+            | Spawn key xform substate0 ->
+               {
+                  ordinal = ordinal';
+                  children = 
+                     Map.add state.children key (substate0, xform)
+               }
+            | Service key subevent ->
+               (match Map.lookup state.children key with
+                  | (substate, xform) ->
+                     let substate' = xform substate subevent in
+                        {
+                           ordinal = ordinal';
+                           children = 
+                              Map.subst state.children key (substate', xform)
+                        })
 
-   (*val init:
-      #key_t: Type -> #substate_t: Type -> #subevent_t: Type ->
-      Tot (trace_g key_t substate_t subevent_t)
-   let init (key_t: Type) (substate_t: Type) (subevent_t: Type) =
-      Subtrace.init 
-         (transform) 
-         ({
-            ordinal = 0;
-            children = Map.empty
-         })*)
+   val init:
+      #key_t: Type 
+      -> #substate_t: Type 
+      -> #subevent_t: Type 
+      -> Tot (trace_g key_t substate_t subevent_t)
+   let init 
+      (key_t: Type) 
+      (substate_t: Type) 
+      (subevent_t: Type) 
+      = 
+         Subtrace.init 
+            (transform) 
+            ({
+               ordinal = 0;
+               children = Map.empty
+            })
 
 // $vim-fst:32: vim:set sts=3 sw=3 et ft=fstar:,$
 
